src/MiscellaneousTypes.v
@@ -1,0 +1,100 @@
+(** MiscellaneousTypes.
+  This file describes various internal data types used in the source of R.
+  In contrary to [InternalTypes], the types described here are fairly independent. **)
+
+(* Copyright © 2020 Martin Bodin
+
+  This program is free software; you can redistribute it and/or modify
+  it under the terms of the GNU General Public License as published by
+  the Free Software Foundation; either version 2 of the License, or
+  (at your option) any later version.
+
+  This program is distributed in the hope that it will be useful,
+  but WITHOUT ANY WARRANTY; without even the implied warranty of
+  MERCHANTABILITY or FITNESS FOR A PARTICULAR PURPOSE.  See the
+  GNU General Public License for more details.
+
+  You should have received a copy of the GNU General Public License
+  along with this program; if not, write to the Free Software
+  Foundation, Inc., 51 Franklin St, Fifth Floor, Boston, MA  02110-1301 USA *)
+
+Require Export Rinternals Common.
+
+(** * [Type2Table] **)
+
+(** These definitions can be found in the file main/util.c. **)
+
+Record Type2Table_type := make_Type2Table_type {
+    Type2Table_cstrName : string ;
+    Type2Table_rcharName : SEXP ;
+    Type2Table_rstrName : SEXP ;
+    Type2Table_rsymName : SEXP ;
+  }.
+
+Instance Type2Table_type_Inhab : Inhab Type2Table_type.
+  apply prove_Inhab. constructors; apply arbitrary.
+Qed.
+
+
+(** * [BindData] **)
+
+(** These definitions can be found in the file main/bind.c. **)
+
+Record BindData := make_BindData {
+    BindData_ans_flags : nbits 10 ;
+    BindData_ans_ptr : SEXP ;
+    BindData_ans_length : nat ;
+    BindData_ans_names : SEXP ;
+    BindData_ans_nnames : nat
+  }.
+
+Definition BindData_with_ans_flags d f := {|
+    BindData_ans_flags := f ;
+    BindData_ans_ptr := BindData_ans_ptr d ;
+    BindData_ans_length := BindData_ans_length d ;
+    BindData_ans_names := BindData_ans_names d ;
+    BindData_ans_nnames := BindData_ans_nnames d
+  |}.
+
+Definition BindData_with_ans_ptr d p := {|
+    BindData_ans_flags := BindData_ans_flags d ;
+    BindData_ans_ptr := p ;
+    BindData_ans_length := BindData_ans_length d ;
+    BindData_ans_names := BindData_ans_names d ;
+    BindData_ans_nnames := BindData_ans_nnames d
+  |}.
+
+Definition BindData_with_ans_length d l := {|
+    BindData_ans_flags := BindData_ans_flags d ;
+    BindData_ans_ptr := BindData_ans_ptr d ;
+    BindData_ans_length := l ;
+    BindData_ans_names := BindData_ans_names d ;
+    BindData_ans_nnames := BindData_ans_nnames d
+  |}.
+
+Definition BindData_with_ans_names d n := {|
+    BindData_ans_flags := BindData_ans_flags d ;
+    BindData_ans_ptr := BindData_ans_ptr d ;
+    BindData_ans_length := BindData_ans_length d ;
+    BindData_ans_names := n ;
+    BindData_ans_nnames := BindData_ans_nnames d
+  |}.
+
+Definition BindData_with_ans_nnames d n := {|
+    BindData_ans_flags := BindData_ans_flags d ;
+    BindData_ans_ptr := BindData_ans_ptr d ;
+    BindData_ans_length := BindData_ans_length d ;
+    BindData_ans_names := BindData_ans_names d ;
+    BindData_ans_nnames := n
+  |}.
+
+
+(** * [pmatch] **)
+
+(** These definitions can be found in the file main/subset.c. **)
+
+Inductive pmatch :=
+  | NO_MATCH
+  | EXACT_MATCH
+  | PARTIAL_MATCH
+  .
