src/.dir-locals.el
@@ -1,6 +1,5 @@
 ((coq-mode . ((coq-load-path . (
         ("." "Main")
         ("../lib/extra" "Lib")
-    	("../lib/tlc/src" "TLC")
     )))))
 
